cleanup: make more predicates agnostic on label type
and add some additional functions and lemmas to reason on the trace

src/core/DY.Core.Trace.Base.fst
@@ -4,6 +4,8 @@ open DY.Core.Trace.Type
 open DY.Core.Bytes.Type
 open DY.Core.Label.Type
 
+#set-options "--fuel 1 --ifuel 1"
+
 /// Shorthands for trace and trace events.
 
 type trace_event = trace_event_ label
@@ -27,7 +29,7 @@ type timestamp = nat
 
 [@@ "opaque_to_smt"]
 val prefix: #label_t:Type -> tr:trace_ label_t -> i:timestamp{i <= length tr} -> trace_ label_t
-let rec prefix tr i =
+let rec prefix #label_t tr i =
   if length tr = i then
     tr
   else
@@ -40,7 +42,7 @@ let rec prefix tr i =
 
 [@@ "opaque_to_smt"]
 val grows: #label_t:Type -> trace_ label_t -> trace_ label_t -> prop
-let grows tr1 tr2 =
+let grows #label_t tr1 tr2 =
   length tr1 <= length tr2 /\
   tr1 == prefix tr2 (length tr1)
 
@@ -72,24 +74,26 @@ let rec grows_induction_principle #label_t p pf tr1 tr2 =
 /// The relation <$ is reflexive.
 
 val grows_reflexive:
-  tr:trace ->
+  #label_t:Type ->
+  tr:trace_ label_t ->
   Lemma (tr <$ tr)
   [SMTPat (tr <$ tr)]
-let grows_reflexive tr =
-  reveal_opaque (`%grows) (grows #label);
-  norm_spec [zeta; delta_only [`%prefix]] (prefix #label)
+let grows_reflexive #label_t tr =
+  reveal_opaque (`%grows) (grows #label_t);
+  norm_spec [zeta; delta_only [`%prefix]] (prefix #label_t)
 
 /// The relation <$ is transitive.
 
 val grows_transitive:
-  tr1:trace -> tr2:trace -> tr3:trace ->
+  #label_t:Type ->
+  tr1:trace_ label_t -> tr2:trace_ label_t -> tr3:trace_ label_t ->
   Lemma
   (requires tr1 <$ tr2 /\ tr2 <$ tr3)
   (ensures tr1 <$ tr3)
   [SMTPat (tr1 <$ tr2); SMTPat (tr1 <$ tr3)]
-let rec grows_transitive tr1 tr2 tr3 =
-  reveal_opaque (`%grows) (grows #label);
-  norm_spec [zeta; delta_only [`%prefix]] (prefix #label);
+let rec grows_transitive #label_t tr1 tr2 tr3 =
+  reveal_opaque (`%grows) (grows #label_t);
+  norm_spec [zeta; delta_only [`%prefix]] (prefix #label_t);
   if length tr2 >= length tr3 then
     ()
   else (
@@ -100,12 +104,13 @@ let rec grows_transitive tr1 tr2 tr3 =
 /// The prefix function outputs traces of the correct length.
 
 val length_prefix:
-  tr:trace -> i:timestamp{i <= length tr} ->
+  #label_t:Type ->
+  tr:trace_ label_t -> i:timestamp{i <= length tr} ->
   Lemma
   (ensures length (prefix tr i) == i)
   [SMTPat (length (prefix tr i))]
-let rec length_prefix tr i =
-  norm_spec [zeta; delta_only [`%prefix]] (prefix #label);
+let rec length_prefix #label_t tr i =
+  norm_spec [zeta; delta_only [`%prefix]] (prefix #label_t);
   if length tr = i then ()
   else
     let Snoc tr_init _ = tr in
@@ -114,29 +119,32 @@ let rec length_prefix tr i =
 /// A trace which is the prefix of another is shorter.
 
 val length_grows:
-  tr1:trace -> tr2:trace ->
+  #label_t:Type ->
+  tr1:trace_ label_t -> tr2:trace_ label_t ->
   Lemma
   (requires tr1 <$ tr2)
   (ensures length tr1 <= length tr2)
   [SMTPat (tr1 <$ tr2)]
-let length_grows tr1 tr2 =
-  reveal_opaque (`%grows) (grows #label)
+let length_grows #label_t tr1 tr2 =
+  reveal_opaque (`%grows) (grows #label_t)
 
 /// The prefix function outputs traces that are prefixes of the input.
 
 val prefix_grows:
-  tr:trace -> i:timestamp{i <= length tr} ->
+  #label_t:Type ->
+  tr:trace_ label_t -> i:timestamp{i <= length tr} ->
   Lemma
   (ensures (prefix tr i) <$ tr)
   //TODO: is this SMTPat dangerous? Should we restrict it to the "safe" on below?
   [SMTPat (prefix tr i)]
   //[SMTPat ((prefix tr i) <$ tr)]
-let prefix_grows tr i =
-  reveal_opaque (`%grows) (grows #label);
-  norm_spec [zeta; delta_only [`%prefix]] (prefix #label)
+let prefix_grows #label_t tr i =
+  reveal_opaque (`%grows) (grows #label_t);
+  norm_spec [zeta; delta_only [`%prefix]] (prefix #label_t)
 
 val prefix_prefix_grows:
-  tr1:trace -> tr2:trace -> i1:timestamp -> i2:timestamp ->
+  #label_t:Type ->
+  tr1:trace_ label_t -> tr2:trace_ label_t -> i1:timestamp -> i2:timestamp ->
   Lemma
   (requires
     tr1 <$ tr2 /\
@@ -150,9 +158,9 @@ val prefix_prefix_grows:
   // [SMTPat (prefix tr1 i1);
   //  SMTPat (prefix tr2 i2);
   //  SMTPat (tr1 <$ tr2)]
-let rec prefix_prefix_grows tr1 tr2 i1 i2 =
-  reveal_opaque (`%grows) (grows #label);
-  norm_spec [zeta; delta_only [`%prefix]] (prefix #label);
+let rec prefix_prefix_grows #label_t tr1 tr2 i1 i2 =
+  reveal_opaque (`%grows) (grows #label_t);
+  norm_spec [zeta; delta_only [`%prefix]] (prefix #label_t);
   if i2 = length tr2 then ()
   else if length tr1 = length tr2 then (
     let Snoc tr1_init _ = tr1 in
@@ -164,7 +172,8 @@ let rec prefix_prefix_grows tr1 tr2 i1 i2 =
   )
 
 val prefix_prefix_eq:
-  tr1:trace -> tr2:trace -> i:timestamp ->
+  #label_t:Type ->
+  tr1:trace_ label_t -> tr2:trace_ label_t -> i:timestamp ->
   Lemma
   (requires
     tr1 <$ tr2 /\
@@ -174,9 +183,9 @@ val prefix_prefix_eq:
   [SMTPat (prefix tr1 i);
    SMTPat (prefix tr2 i);
    SMTPat (tr1 <$ tr2)]
-let rec prefix_prefix_eq tr1 tr2 i =
-  reveal_opaque (`%grows) (grows #label);
-  norm_spec [zeta; delta_only [`%prefix]] (prefix #label);
+let rec prefix_prefix_eq #label_t tr1 tr2 i =
+  reveal_opaque (`%grows) (grows #label_t);
+  norm_spec [zeta; delta_only [`%prefix]] (prefix #label_t);
   if length tr1 = length tr2 then ()
   else (
     let Snoc tr2_init _ = tr2 in
@@ -191,7 +200,7 @@ val get_event_at:
   #label_t:Type ->
   tr:trace_ label_t -> i:timestamp{i < length tr} ->
   trace_event_ label_t
-let rec get_event_at tr i =
+let rec get_event_at #label_t tr i =
   if i+1 = length tr then
     let Snoc _ last = tr in
     last
@@ -206,11 +215,9 @@ val event_at:
   #label_t:Type ->
   trace_ label_t -> timestamp -> trace_event_ label_t ->
   prop
-let event_at tr i e =
-  if i >= length tr then
-    False
-  else
-    e == get_event_at tr i
+let event_at #label_t tr i e =
+  i < length tr /\
+  e == get_event_at tr i
 
 /// Has some particular event been triggered in the trace (at any timestamp)?
 
@@ -218,10 +225,28 @@ val event_exists:
   #label_t:Type ->
   trace_ label_t -> trace_event_ label_t ->
   prop
-let event_exists tr e =
+let event_exists #label_t tr e =
   exists i. event_at tr i e
 
 /// An event in the trace stays here when the trace grows.
+
+val get_event_at_grows:
+  #label_t:Type ->
+  tr1:trace_ label_t -> tr2:trace_ label_t ->
+  i:timestamp{i < length tr1} ->
+  Lemma
+  (requires tr1 <$ tr2)
+  (ensures get_event_at tr1 i == get_event_at tr2 i)
+  [SMTPat (get_event_at tr1 i); SMTPat (tr1 <$ tr2)]
+let rec get_event_at_grows #label_t tr1 tr2 i =
+  reveal_opaque (`%grows) (grows #label_t);
+  norm_spec [zeta; delta_only [`%prefix]] (prefix #label_t);
+  if i >= length tr1 then ()
+  else if length tr1 >= length tr2 then ()
+  else (
+    let Snoc tr2_init _ = tr2 in
+    get_event_at_grows tr1 tr2_init i
+  )
 
 val event_at_grows:
   #label_t:Type ->
@@ -231,63 +256,138 @@ val event_at_grows:
   (requires event_at tr1 i e /\ tr1 <$ tr2)
   (ensures event_at tr2 i e)
   [SMTPat (event_at tr1 i e); SMTPat (tr1 <$ tr2)]
-let rec event_at_grows #label_t tr1 tr2 i e =
-  reveal_opaque (`%grows) (grows #label_t);
-  norm_spec [zeta; delta_only [`%prefix]] (prefix #label_t);
-  if i >= length tr1 then ()
-  else if length tr1 >= length tr2 then ()
-  else (
-    let Snoc tr2_init _ = tr2 in
-    event_at_grows tr1 tr2_init i e
-  )
+let event_at_grows #label_t tr1 tr2 i e = ()
 
 /// Shorthand predicates.
 
 /// Has a message been sent on the network?
 
-val msg_sent_on_network: trace -> bytes -> prop
-let msg_sent_on_network tr msg =
+val msg_sent_on_network:
+  #label_t:Type ->
+  trace_ label_t -> bytes ->
+  prop
+let msg_sent_on_network #label_t tr msg =
   event_exists tr (MsgSent msg)
 
 /// Has some state been stored by a principal?
 
-val state_was_set: trace -> principal -> state_id -> bytes -> prop
-let state_was_set tr prin sess_id content =
+val state_was_set:
+  #label_t:Type ->
+  trace_ label_t -> principal -> state_id -> bytes ->
+  prop
+let state_was_set #label_t tr prin sess_id content =
   event_exists tr (SetState prin sess_id content)
 
 /// Has a principal been corrupt?
 
-val was_corrupt: #label_t:Type -> trace_ label_t -> principal -> state_id -> prop
-let was_corrupt tr prin sess_id =
+val was_corrupt:
+  #label_t:Type ->
+  trace_ label_t -> principal -> state_id ->
+  prop
+let was_corrupt #label_t tr prin sess_id =
   event_exists tr (Corrupt prin sess_id)
 
 /// Has a (custom, protocol-specific) event been triggered at some timestamp?
 
-val event_triggered_at: trace -> timestamp -> principal -> string -> bytes -> prop
-let event_triggered_at tr i prin tag content =
+val event_triggered_at:
+  #label_t:Type ->
+  trace_ label_t -> timestamp -> principal -> string -> bytes ->
+  prop
+let event_triggered_at #label_t tr i prin tag content =
   event_at tr i (Event prin tag content)
 
 /// Has a (custom, protocol-specific) event been triggered (at any timestamp)?
 
-val event_triggered: trace -> principal -> string -> bytes -> prop
-let event_triggered tr prin tag content =
+val event_triggered:
+  #label_t:Type ->
+  trace_ label_t -> principal -> string -> bytes ->
+  prop
+let event_triggered #label_t tr prin tag content =
   exists i. event_triggered_at tr i prin tag content
+
+/// Find the timestamp at which an event has been triggered.
+/// (Can be useful when debugging a proof.)
+
+#push-options "--ifuel 1 --fuel 2 --z3rlimit 25"
+val find_event_triggered_at_timestamp_opt:
+  #label_t:Type ->
+  tr:trace_ label_t -> prin:principal -> tag:string -> content:bytes ->
+  Pure (option timestamp)
+  (requires True)
+  (ensures fun opt_i ->
+    match opt_i with
+    | Some i ->
+      event_triggered_at tr i prin tag content /\
+      ~(event_triggered (prefix tr i) prin tag content)
+    | None -> ~(event_triggered tr prin tag content)
+  )
+let rec find_event_triggered_at_timestamp_opt #label_t tr prin tag content =
+  match tr with
+  | Nil -> None
+  | Snoc init last ->
+    match find_event_triggered_at_timestamp_opt init prin tag content with
+    | Some i -> Some i
+    | None -> (
+      match last with
+      | Event prin' tag' content' ->
+        if prin = prin' && tag = tag' && content = content' then
+          Some (length init)
+        else None
+      | _ -> None
+    )
+#pop-options
+
+[@@ "opaque_to_smt"]
+val find_event_triggered_at_timestamp:
+  #label_t:Type ->
+  tr:trace_ label_t -> prin:principal -> tag:string -> content:bytes ->
+  Pure timestamp
+  (requires event_triggered tr prin tag content)
+  (ensures fun i ->
+    event_triggered_at tr i prin tag content /\
+    ~(event_triggered (prefix tr i) prin tag content)
+  )
+let find_event_triggered_at_timestamp #label_t tr prin tag content =
+  Some?.v (find_event_triggered_at_timestamp_opt tr prin tag content)
+
+val find_event_triggered_at_timestamp_later:
+  #label_t:Type ->
+  tr1:trace_ label_t -> tr2:trace_ label_t ->
+  prin:principal -> tag:string -> content:bytes ->
+  Lemma
+  (requires
+    event_triggered tr1 prin tag content /\
+    tr1 <$ tr2
+  )
+  (ensures find_event_triggered_at_timestamp tr1 prin tag content == find_event_triggered_at_timestamp tr2 prin tag content)
+let rec find_event_triggered_at_timestamp_later #label_t tr1 tr2 prin tag content =
+  if length tr1 = length tr2 then ()
+  else (
+    reveal_opaque (`%grows) (grows #label_t);
+    norm_spec [zeta; delta_only [`%prefix]] (prefix #label_t);
+    let Snoc init2 last2 = tr2 in
+    find_event_triggered_at_timestamp_later tr1 init2 prin tag content
+  )
 
 /// An event being triggered at some time stays triggered as the trace grows.
 
 val event_triggered_grows:
-  tr1:trace -> tr2:trace ->
+  #label_t:Type ->
+  tr1:trace_ label_t -> tr2:trace_ label_t ->
   prin:principal -> tag:string -> content:bytes  ->
   Lemma
   (requires event_triggered tr1 prin tag content /\ tr1 <$ tr2)
   (ensures event_triggered tr2 prin tag content)
   [SMTPat (event_triggered tr1 prin tag content); SMTPat (tr1 <$ tr2)]
-let event_triggered_grows tr1 tr2 prin tag content = ()
+let event_triggered_grows #label_t tr1 tr2 prin tag content = ()
 
 /// Has a random bytestring been generated at some timestamp?
 
-val rand_generated_at: trace -> timestamp -> bytes -> prop
-let rand_generated_at tr i b =
+val rand_generated_at:
+  #label_t:Type ->
+  trace_ label_t -> timestamp -> bytes ->
+  prop
+let rand_generated_at #label_t tr i b =
   match b with
   | Rand usg len time ->
     time == i /\ (exists lab. event_at tr i (RandGen usg lab len))
@@ -323,23 +423,21 @@ val fmap_trace:
   #a:Type -> #b:Type ->
   (a -> b) -> trace_ a ->
   trace_ b
-let rec fmap_trace f tr =
+let rec fmap_trace #a #b f tr =
   match tr with
   | Nil -> Nil
   | Snoc init last ->
     Snoc (fmap_trace f init) (fmap_trace_event f last)
 
-val forget_label:
+val length_fmap_trace:
   #a:Type -> #b:Type ->
-  b ->
-  a -> b
-let forget_label #a #b x _ = x
-
-val trace_forget_labels:
-  trace ->
-  trace_ unit
-let trace_forget_labels tr =
-  fmap_trace (forget_label ()) tr
+  f:(a -> b) -> tr:trace_ a ->
+  Lemma (length (fmap_trace f tr) == length tr)
+  [SMTPat (length (fmap_trace f tr))]
+let rec length_fmap_trace #a #b f tr =
+  match tr with
+  | Nil -> ()
+  | Snoc init last -> length_fmap_trace f init
 
 val fmap_trace_identity:
   #a:Type ->
@@ -367,29 +465,71 @@ let rec fmap_trace_compose #a #b #c f g h tr =
   | Snoc init last ->
     fmap_trace_compose f g h init
 
-val length_trace_forget_labels:
-  tr:trace ->
-  Lemma (length (trace_forget_labels tr) == length tr)
-let rec length_trace_forget_labels tr =
-  match tr with
-  | Nil -> ()
-  | Snoc init last -> length_trace_forget_labels init
+val fmap_trace_prefix:
+  #a:Type -> #b:Type ->
+  f:(a -> b) ->
+  tr:trace_ a -> i:timestamp{i <= length tr} ->
+  Lemma (
+    prefix (fmap_trace f tr) i == fmap_trace f (prefix tr i)
+  )
+let rec fmap_trace_prefix #a #b f tr i =
+  norm_spec [zeta; delta_only [`%prefix]] (prefix #a);
+  norm_spec [zeta; delta_only [`%prefix]] (prefix #b);
+  if length tr = i then ()
+  else
+    let Snoc tr_init _ = tr in
+    fmap_trace_prefix f tr_init i
 
-val trace_forget_labels_later:
-  tr1:trace -> tr2:trace ->
+val fmap_trace_later:
+  #a:Type -> #b:Type ->
+  f:(a -> b) ->
+  tr1:trace_ a -> tr2:trace_ a ->
   Lemma
   (requires tr1 <$ tr2)
-  (ensures (trace_forget_labels tr1) <$ (trace_forget_labels tr2))
-let rec trace_forget_labels_later tr1 tr2 =
-  reveal_opaque (`%grows) (grows #unit);
-  norm_spec [zeta; delta_only [`%prefix]] (prefix #unit);
-  reveal_opaque (`%grows) (grows #label);
-  norm_spec [zeta; delta_only [`%prefix]] (prefix #label);
-  if length tr1 = length tr2 then (
-    match tr1, tr2 with
-    | Nil, Nil -> ()
-    | Snoc tr1_init _, Snoc tr2_init _ -> ()
-  ) else (
-    let Snoc tr2_init tr2_last = tr2 in
-    trace_forget_labels_later tr1 tr2_init
+  (ensures (fmap_trace f tr1) <$ (fmap_trace f tr2))
+let fmap_trace_later #a #b f tr1 tr2 =
+  reveal_opaque (`%grows) (grows #a);
+  reveal_opaque (`%grows) (grows #b);
+  fmap_trace_prefix f tr2 (length tr1)
+
+val fmap_trace_recover_before:
+  #a:Type -> #b:Type ->
+  f:(a -> b) ->
+  tr1:trace_ b -> tr2:trace_ a ->
+  Pure (trace_ a)
+  (requires
+    tr1 <$ fmap_trace f tr2
   )
+  (ensures fun tr1' ->
+    tr1 == fmap_trace f tr1' /\
+    tr1' <$ tr2
+  )
+let fmap_trace_recover_before #a #b f tr1 tr2 =
+  reveal_opaque (`%grows) (grows #b);
+  fmap_trace_prefix f tr2 (length tr1);
+  prefix tr2 (length tr1)
+
+val get_event_at_fmap_trace:
+  #a:Type -> #b:Type ->
+  f:(a -> b) -> tr:trace_ a -> i:timestamp{i < length tr} ->
+  Lemma (
+    get_event_at (fmap_trace f tr) i == fmap_trace_event f (get_event_at tr i)
+  )
+let rec get_event_at_fmap_trace #a #b f tr i =
+  if i+1 = length tr then ()
+  else (
+    let Snoc tr_init _ = tr in
+    get_event_at_fmap_trace f tr_init i
+  )
+
+val forget_label:
+  #a:Type -> #b:Type ->
+  b ->
+  a -> b
+let forget_label #a #b x _ = x
+
+val trace_forget_labels:
+  trace ->
+  trace_ unit
+let trace_forget_labels tr =
+  fmap_trace (forget_label ()) tr
